iris/WpKfree.v
@@ -463,12 +463,12 @@ Section Kfree.
     assert (Hpp10 : add_vec_int (mword_of_int (KF + 0x0c) : mword 64) 4 = mword_of_int (KF + 0x10)) by (apply bv_eq; vm_compute; reflexivity).
     iEval (rewrite Hpp10) in "Hpc".
     (* +0x10 addi a5,a5,-1260  (a5 := <end> = 0x80023558) *)
-    iApply (wp_addi4_s_scfg root_ppn γc Φ (mword_of_int (KF + 0x10)) (mword_of_int 15 : mword 5) (mword_of_int 15 : mword 5) (mword_of_int 0xb14 : mword 12)
+    iApply (wp_addi4_s_scfg root_ppn γc Φ (mword_of_int (KF + 0x10)) (mword_of_int 15 : mword 5) (mword_of_int 15 : mword 5) (mword_of_int 0xb06 : mword 12)
               R3 (dq:=DfracOwn 1)
  ltac:(vm_compute; discriminate)
               with "Hcfg Htlbinv Hpc Hfile Hi10 [-]").
     iIntros "Hcfg Htlbinv Hpc Hfile".
-    set (R4 := <[Regidx (mword_of_int 15 : mword 5) := regval_into_reg (add_vec (R3 !!! Regidx (mword_of_int 15 : mword 5)) (sign_extend' 64 (mword_of_int 0xb14 : mword 12)))]> R3).
+    set (R4 := <[Regidx (mword_of_int 15 : mword 5) := regval_into_reg (add_vec (R3 !!! Regidx (mword_of_int 15 : mword 5)) (sign_extend' 64 (mword_of_int 0xb06 : mword 12)))]> R3).
     assert (Hpp14 : add_vec_int (mword_of_int (KF + 0x10) : mword 64) 4 = mword_of_int (KF + 0x14)) by (apply bv_eq; vm_compute; reflexivity).
     iEval (rewrite Hpp14) in "Hpc".
     (* a0 (= the page p) and a5 (= <end>) after the prologue+auipc/addi *)
@@ -759,12 +759,12 @@ Section Kfree.
     assert (Hpp3a : add_vec_int (mword_of_int (KF + 0x36) : mword 64) 4 = mword_of_int (KF + 0x3a)) by (apply bv_eq; vm_compute; reflexivity).
     iEval (rewrite Hpp3a) in "Hpc".
     (* +0x3a addi s2,s2,-1862  (s2 := &kmem) *)
-    iApply (wp_addi4_s_scfg root_ppn γc Φ (mword_of_int (KF + 0x3a)) (mword_of_int 18 : mword 5) (mword_of_int 18 : mword 5) (mword_of_int 0x8ba : mword 12)
+    iApply (wp_addi4_s_scfg root_ppn γc Φ (mword_of_int (KF + 0x3a)) (mword_of_int 18 : mword 5) (mword_of_int 18 : mword 5) (mword_of_int 0x8ac : mword 12)
               S1 (dq:=DfracOwn 1)
  ltac:(vm_compute; discriminate)
               with "Hcfg Htlbinv Hpc Hfile Hi3a [-]").
     iIntros "Hcfg Htlbinv Hpc Hfile".
-    set (S2 := <[Regidx (mword_of_int 18 : mword 5) := regval_into_reg (add_vec (S1 !!! Regidx (mword_of_int 18 : mword 5)) (sign_extend' 64 (mword_of_int 0x8ba : mword 12)))]> S1).
+    set (S2 := <[Regidx (mword_of_int 18 : mword 5) := regval_into_reg (add_vec (S1 !!! Regidx (mword_of_int 18 : mword 5)) (sign_extend' 64 (mword_of_int 0x8ac : mword 12)))]> S1).
     assert (Hs2kmem : S2 !!! Regidx (mword_of_int 18 : mword 5) = mword_of_int KernelSyms.kmem).
     { rewrite /S2 lookup_total_insert. rewrite /S1 lookup_total_insert. apply bv_eq; vm_compute; reflexivity. }
     assert (Hpp3e : add_vec_int (mword_of_int (KF + 0x3a) : mword 64) 4 = mword_of_int (KF + 0x3e)) by (apply bv_eq; vm_compute; reflexivity).
