iris/WpMmodeJalr.v
@@ -224,4 +224,98 @@ Section RvcRet.
     iSplitR; [ iPureIntro; exact Hdom | iExact "Hfmap" ].
   Qed.
 
+  (* [wp_cret_gpr] for a merely 2-aligned return target.  Under the C extension
+     (misa.C, held by [mmode_config]'s [hw_config]) the model's jalr accepts a
+     2-aligned target, so this needs only [is_aligned_paddr .. 2] where the
+     4-aligned leaf needs [.. 4].  Needed after an odd-halfword layout shift
+     flips a callee's return-address parity (e.g. start()'s ADUE write pushing
+     the timerinit call to a 2-aligned return). *)
+  Lemma wp_cret_gpr_zca (Φ : mval -> iProp Σ) (pc : mword 64) (ra : mword 5)
+      (m : gmap regidx (mword 64)) (pmpcfg0 : type_of_register pmpcfg_n) (q : Qp) :
+    pmp_allows_all pmpcfg0 ->
+    uint ra <> 0 ->
+    is_aligned_paddr (Physaddr (cret_target (m !!! Regidx ra))) 2 = true ->
+    mmode_config (DfracOwn q) -∗
+    pmpcfg_n ↦ᵣ{DfracOwn q} pmpcfg0 -∗
+    pc_is pc -∗
+    gpr_file m -∗
+    instr pc true (JALR (zeros' 12, Regidx ra, zreg)) -∗
+    ( mmode_config (DfracOwn q) -∗
+      pmpcfg_n ↦ᵣ{DfracOwn q} pmpcfg0 -∗
+      pc_is (cret_target (m !!! Regidx ra)) -∗
+      gpr_file m -∗
+      WP (Loop : expr riscv_lang) {{ Φ }}) -∗
+    WP (Loop : expr riscv_lang) {{ Φ }}.
+  Proof.
+    iIntros (Hpmp Hra Halign) "Hmm Hpmpc [Hpc Hnpc] [%Hdom Hfmap] Hinstr Hcont".
+    pose proof (aligned2_jump_bit _ Halign) as Hal0.
+    iDestruct (mmode_config_split with "Hmm") as "[Hmm_wp Hmm_k]".
+    iDestruct "Hmm_k" as "(#Hhw & #Hinv & Hhs_k & Hpriv_k & Hmst_k)".
+    iPoseProof "Hhw" as "#Hhwc".
+    iDestruct "Hhwc" as (misa0 mseccfg0 pmar0 elp0)
+      "(#Hmisa & #Hmseccfg & #Hpma & #Hhtif & #Help & %HmisaS & %HmisaC &
+        %HmisaU & %HmisaM & %Hpma_all & %Hseccfg1 & %Hmlpe & %Help_np & %HmisaA & %Hmisa_val0 & %Hmseccfg_val0)".
+    iDestruct "Hpmpc" as "[Hpmpc_wp Hpmpc_k]".
+    iApply (wp_instr Φ pc true (JALR (zeros' 12, Regidx ra, zreg)) pmpcfg0
+              Hpmp with "Hmm_wp Hpmpc_wp Hpc Hinstr").
+    iIntros (σ Hpceq) "Hsi".
+    iDestruct "Hsi" as "[Hreg Hmem]".
+    assert (Hm1 : m !! Regidx ra = Some (m !!! Regidx ra))
+      by (apply lookup_lookup_total_dom; apply Hdom).
+    iDestruct (reg_valid_dq with "Hreg Hpriv_k")  as %Lpriv.
+    iDestruct (reg_valid_dq with "Hreg Hmseccfg") as %Lsec.
+    iDestruct (reg_valid_dq with "Hreg Hmisa")    as %Lmisa.
+    iMod (reg_update _ nextPC _ (add_vec_int pc 2) with "Hreg Hnpc") as "[Hreg Hnpc]".
+    set (s_pc := set_reg σ nextPC (add_vec_int pc 2)).
+    iDestruct (big_sepM_lookup_acc _ _ _ _ Hm1 with "Hfmap") as "[Hr1c Hfb1]".
+    iDestruct (gpr_pt_value ra (m !!! Regidx ra) s_pc with "Hreg Hr1c") as %Hrv.
+    iDestruct ("Hfb1" with "Hr1c") as "Hfmap".
+    assert (Lrav : register_lookup (R_bitvector_64 (gpr_of_Z (uint ra))) s_pc.(sregs)
+                   = m !!! Regidx ra).
+    { rewrite -Hrv. replace (Z.eqb (uint ra) 0) with false
+        by (symmetry; apply Z.eqb_neq; exact Hra). reflexivity. }
+    assert (Hzic : exec (currentlyEnabled Ext_Zicfilp) s_pc = Some (false, s_pc)).
+    { apply exec_cE_zicfilp_false.
+      - unfold s_pc; tmig; exact Lpriv.
+      - unfold s_pc; tmig; rewrite Lsec; exact Hmlpe. }
+    assert (Hzca : exec (currentlyEnabled Ext_Zca) s_pc = Some (true, s_pc)).
+    { apply exec_currentlyEnabled_Zca. unfold s_pc; tmig; rewrite Lmisa; exact HmisaC. }
+    assert (Htgt : update_vec_dec (add_vec
+                     (register_lookup (R_bitvector_64 (gpr_of_Z (uint ra))) s_pc.(sregs))
+                     (sign_extend' 64 (zeros' 12 : mword 12))) 0 ('b"0")
+                   = cret_target (m !!! Regidx ra)).
+    { unfold cret_target. rewrite Lrav. reflexivity. }
+    assert (Hexec_spc :
+      exec (execute (JALR (zeros' 12, Regidx ra, zreg))) s_pc
+      = Some (RETIRE_SUCCESS, set_reg s_pc nextPC (cret_target (m !!! Regidx ra)))).
+    { change (execute (JALR (zeros' 12, Regidx ra, zreg)))
+        with (execute_JALR (zeros' 12) (Regidx ra) zreg).
+      change zreg with (Regidx cli_rs1).
+      rewrite (exec_execute_JALR_ret_zca (zeros' 12) ra cli_rs1 s_pc Hra
+                 ltac:(vm_compute; reflexivity) Hzic Hzca
+                 ltac:(rewrite Htgt; exact Hal0)).
+      rewrite Htgt. reflexivity. }
+    iMod (reg_update _ nextPC _ (cret_target (m !!! Regidx ra)) with "Hreg Hnpc") as "[Hreg Hnpc]".
+    iModIntro.
+    iExists (set_reg s_pc nextPC (cret_target (m !!! Regidx ra))).
+    iSplitR.
+    { iPureIntro. rewrite Hpceq.
+      change (if true then 2%Z else 4%Z) with 2%Z. fold s_pc. exact Hexec_spc. }
+    iSplitL "Hreg Hmem".
+    { unfold s_pc, set_reg; cbn [sregs mem]. iFrame "Hreg Hmem". }
+    iIntros "Hmm' Hpmpc' Hpc'".
+    assert (Lnpc : register_lookup nextPC
+             (set_reg s_pc nextPC (cret_target (m !!! Regidx ra))).(sregs)
+             = cret_target (m !!! Regidx ra)).
+    { rewrite register_lookup_set. reflexivity. }
+    iEval (rewrite Lnpc) in "Hpc'".
+    iAssert (mmode_config (DfracOwn (q/2)))%I
+      with "[Hhs_k Hpriv_k Hmst_k]" as "Hmm_k'".
+    { iFrame "Hhw Hinv Hhs_k Hpriv_k Hmst_k". }
+    iDestruct (mmode_config_combine with "Hmm' Hmm_k'") as "Hmm''".
+    iCombine "Hpmpc' Hpmpc_k" as "Hpmpc''".
+    iApply ("Hcont" with "Hmm'' Hpmpc'' [$Hpc' $Hnpc] [Hfmap]").
+    iSplitR; [ iPureIntro; exact Hdom | iExact "Hfmap" ].
+  Qed.
+
 End RvcRet.
